%
% Quiz 23 : 2019-08-07 (W)
%
% Exercise 8.2.12 (p 483) in Farlow et al.
%
\section{Exercise}

(5 pt) Solve the following nonhomogeneous 2nd-order linear initial value problem:
\begin{align*}
y'' + y' + y
=
e^{-t},
&&
y(0)
=
0,
&&
y'(0)
=
1.
\end{align*}
\fontHint{Recall that, from the definition of the lapace transform,
\begin{align*}
\laplaceTransform\{y'\}(s)
=
s \laplaceTransform\{y\} - y(0).
\end{align*}
Applying this result to $y''$, we get
\begin{align*}
\laplaceTransform\{y''\}(s)
=
s \laplaceTransform\{y'\} - y'(0)
=
s^{2} \laplaceTransform\{y\} - s y(0) - y'(0).
\end{align*}
The following transform--inverse-transform pairs may be useful:
\begin{align*}
\laplaceTransform\{e^{a t}\}
=
\frac{1}{s - a},
\end{align*}}

\spaceSolution{5in}{% Begin solution.
Applying the laplace transform to both sides of the ODE, and using the fact that the laplace transform is linear, we get
\begin{align}
\laplaceTransform\{y''\} + \laplaceTransform\{y'\} + \laplaceTransform\{y\}
=
\laplaceTransform\{y'' + y' + y\}
=
\laplaceTransform\{e^{-t}\}.%
\label{eq : Quiz23 Initial Application Laplace Transform}
\end{align}
Denote
\begin{align*}
Y(s)
=
\laplaceTransform\{y\}.
\end{align*}
From the definition of the laplace transform, and using the given initial conditions, we compute
\begin{align*}
\laplaceTransform\{y'\}
&=
s \laplaceTransform\{y\} - y(0)
=
s Y(s) - 0
=
s Y(s)
\\
\laplaceTransform\{y''\}
&=
s^{2} \laplaceTransform\{y'\} - s f(0) - f'(0)
=
s^{2} Y(s) - 1.
\end{align*}
Substituting these results into \eqref{eq : Quiz23 Initial Application Laplace Transform}, we get
\begin{align*}
\left(s^{2} Y(s) - 1\right) + s Y(s) + Y(s)
=
\laplaceTransform\{e^{-t}\}
=
\frac{1}{s + 1}.
\end{align*}
Solving this equation for $Y(s)$, we get
\begin{align*}
Y(s)
=
\frac{\frac{1}{s + 1} + 1}{s^{2} + s + 1}
=
\frac{\frac{s + 2}{s + 1}}{s^{2} + s + 1}
=
\frac{s + 2}{(s + 1) (s^{2} + s + 1)}.
\end{align*}
Setting up the partial fraction decomposition, we have
\begin{align*}
\frac{s + 2}{(s + 1) (s^{2} + s + 1)}
=
\frac{A}{s + 1} + \frac{B s + C}{s^{2} + s + 1}.
\end{align*}
Clearing denominators, we get
\begin{align*}
s + 2
=
(s^{2} + s + 1) A + (s + 1) (B s + C).
\end{align*}
Now we plug in (at least) three values for $t$ to get a system of equations we can use to solve for $A,B,C$:
\begin{align*}
s = -1
&:
1
=
A
\\
s = 0
&:
2
=
A + C
=
1 + C
\Rightarrow
C
=
1
\\
s = 1
&:
3
=
3 A + 2 (B + C)
=
3 + 2 B + 2
\Rightarrow
B
=
-1.
\end{align*}
Thus
\begin{align*}
Y(s)
&=
\frac{s + 2}{(s + 1) (s^{2} + s + 1)}
\\
&=
\frac{1}{s + 1} + \frac{-s + 1}{s^{2} + s + 1}
\\
&=
\frac{1}{s + 1} - \frac{s - \frac{1}{2}}{(s + \frac{1}{2})^{2} + \frac{3}{4}}
\\
&=
\frac{1}{s + 1} - \frac{s + \frac{1}{2} - 1}{(s + \frac{1}{2})^{2} + \frac{3}{4}}
\\
&=
\frac{1}{s + 1} - \frac{s + \frac{1}{2}}{(s + \frac{1}{2})^{2} + \frac{3}{4}} - \frac{4}{3} \frac{\frac{3}{4}}{(s + \frac{1}{2})^{2} + \frac{3}{4}},
\end{align*}
where
\begin{itemize}
\item in the third equality, in the second term, we have (i) factored out a $-1$ from the numerator and (ii) completed the square in the denominator;
\item in the fourth equality, we have rewritten the numerator so we get the same $s + a$ term as appears in the completed square in the denominator (to set us up for the inverse laplace transform); and
\item in the fifth equality, we have explicitly decomposed the second term into two terms, and rewritten the numerator of our second term (factoring out a $\frac{4}{3}$) so that all terms have a form that appear in our dictionary of transform--inverse-transform pairs.
\end{itemize}
Applying the inverse laplace transform to both sides, and using the fact that it is linear, we get
\begin{align*}
y(t)
&=
\laplaceTransform^{-1}\{\laplaceTransform\{y\}\}
=
\laplaceTransform^{-1}\{Y(s)\}
=
\laplaceTransform^{-1}\left\{\frac{1}{s + 1} - \frac{s + \frac{1}{2}}{(s + \frac{1}{2})^{2} + \frac{3}{4}} - \frac{1}{(s + \frac{1}{2})^{2} + \frac{3}{4}}\right\}
\\
&=
\laplaceTransform^{-1}\left\{\frac{1}{s + 1}\right\} - \laplaceTransform^{-1}\left\{\frac{s + \frac{1}{2}}{(s + \frac{1}{2})^{2} + \frac{3}{4}}\right\} - \laplaceTransform^{-1}\left\{\frac{1}{(s + \frac{1}{2})^{2} + \frac{3}{4}}\right\}
\\
&=
e^{-t} - e^{}
\end{align*}}% End solution.