\section{Exercise}

(5 pt) Let $R \subseteq \reals^{2}$ be the square bounded by the lines
\begin{align*}
x + y
&=
-1,
&
x + y
&=
1,
&
x - y
&=
-1,
&
x - y
&=
1.
\end{align*}
Show that
\begin{align*}
\iint_{R} e^{x + y} \, \intd A
=
e - \frac{1}{e}.
\end{align*}
\fontHint{Apply a change of variables. More precisely, let the equations of the boundary of the region $R$ and the integrand guide your definition of new variables $u,v$ as functions of the given variables $x,y$. Solve for $x,y$ as functions of $u,v$. Remember the Jacobian determinant.}

\spaceSolution{5in}{% Begin solution.
The equations defining the region $R$ (and the integrand) suggest the change of variables
\begin{align*}
u
&=
x + y,
&
v
&=
x - y.
\end{align*}
Solving this system of equations for $x,y$ in terms of $u,v$, we find
\begin{align*}
x
&=
\frac{1}{2} u + \frac{1}{2} v,
&
y
&=
\frac{1}{2} u - \frac{1}{2} v.
\end{align*}
Thus the relevant transformation $T: \reals^{2} \rightarrow \reals^{2}$, from the $u v$-plane to the $x y$-plane, is
\begin{align*}
T(u,v)
=
\left(x(u,v),y(u,v)\right)
=
\left(\frac{1}{2} u + \frac{1}{2} v,\frac{1}{2} u - \frac{1}{2} v\right),
\end{align*}
with Jacobian matrix and Jacobian determinant
\begin{align*}
\jacobian_{T}(u,v)
&=
\begin{pmatrix}
\frac{\partial x}{\partial u}	&	\frac{\partial x}{\partial v}	\\
\frac{\partial y}{\partial u}	&	\frac{\partial y}{\partial u}
\end{pmatrix}
=
\begin{pmatrix}
\frac{1}{2}	&	\frac{1}{2}	\\
\frac{1}{2}	&	-\frac{1}{2}
\end{pmatrix}
&
&\text{and}
&
\det \jacobian_{T}
&=
-\frac{1}{4} - \frac{1}{4}
=
-\frac{1}{2}.
\end{align*}
respectively.

The region $S$ of the $u v$-plane that maps to the region $R$ of the $x y$-plane can be found by rewriting the equations defining $R$ in terms of $u,v$. Doing this, we find
\begin{align*}
S
=
\left\{(u,v) \in \reals^{2} \st -1 \leq u \leq 1,-1 \leq v \leq 1\right\}.
\end{align*}
Applying the change-of-variables theorem to the given integral using the transformation $T$ gives
\begin{align*}
\iint_{R} f(x,y) \, \intd A
&=
\iint_{S} f(T(u,v)) \abs{\det \jacobian_{T}} \, \intd A
\\
&=
\frac{1}{2} \int_{v = -1}^{v = 1} \int_{u = -1}^{u = 1} e^{u} \, \intd u \, \intd v
\\
&=
\frac{1}{2} \int_{v = -1}^{v = 1} \intd v \int_{u = -1}^{u = 1} e^{u} \, \intd u
\\
&=
\frac{1}{2} [2] \left[e^{1} - e^{-1}\right]
=
e - \frac{1}{e}.
\end{align*}
}% End solution.